src/cbor/pulse/raw/everparse/CBOR.Pulse.Raw.EverParse.Det.Impl.Aux.fsti
@@ -79,3 +79,36 @@ val length_det_raw_map_entries
 : Lemma
     (List.Tot.length (det_raw_map_entries l) == List.Tot.length l)
     [SMTPat (List.Tot.length (det_raw_map_entries l))]
+
+(* For map iterator next: convert raw map entry (pair of raw_data_item) back
+   to the spec pair (cbor & cbor). *)
+
+val list_map_mk_cbor_mk_det_raw_cbor_map_entry (l: list (Spec.cbor & Spec.cbor))
+: Lemma (ensures (
+    List.Tot.map SpecRaw.mk_cbor_map_entry (det_raw_map_entries l) == l
+  ))
+
+val list_map_mk_det_raw_cbor_correct_map_entries (l: list (Spec.cbor & Spec.cbor))
+: Lemma (ensures (
+    let l' = det_raw_map_entries l in
+    List.Tot.for_all
+      (CBOR.Spec.Util.holds_on_pair Optimal.raw_data_item_ints_optimal) l' /\
+    List.Tot.for_all
+      (CBOR.Spec.Util.holds_on_pair (Optimal.raw_data_item_sorted Format.deterministically_encoded_cbor_map_key_order)) l'
+  ))
+
+val det_raw_map_entries_inverse (l: list (SpecRawBase.raw_data_item & SpecRawBase.raw_data_item))
+: Lemma
+    (requires
+      List.Tot.for_all
+        (CBOR.Spec.Util.holds_on_pair Optimal.raw_data_item_ints_optimal) l /\
+      List.Tot.for_all
+        (CBOR.Spec.Util.holds_on_pair (Optimal.raw_data_item_sorted Format.deterministically_encoded_cbor_map_key_order)) l)
+    (ensures det_raw_map_entries (List.Tot.map SpecRaw.mk_cbor_map_entry l) == l)
+
+val mk_det_raw_cbor_map_entry_mk_cbor_map_entry (x: SpecRawBase.raw_data_item & SpecRawBase.raw_data_item)
+: Lemma
+    (requires
+      CBOR.Spec.Util.holds_on_pair Optimal.raw_data_item_ints_optimal x /\
+      CBOR.Spec.Util.holds_on_pair (Optimal.raw_data_item_sorted Format.deterministically_encoded_cbor_map_key_order) x)
+    (ensures (SpecRaw.mk_det_raw_cbor_map_entry (SpecRaw.mk_cbor_map_entry x) == x))
